refactor

theories/base.v
@@ -150,41 +150,36 @@ Class MonoPred {A : Type} (F : (A → Prop) → (A → Prop)) := {
 }.
 Global Arguments mono_pred {_ _ _} _ _.
 
-Definition least_fixpoint {A : Type}
+Definition prop_least_fixpoint {A : Type}
     (F : (A → Prop) → (A → Prop)) (x : A) : Prop :=
   tc_opaque (∀ Φ : A -> Prop, (∀ x, F Φ x → Φ x) → Φ x).
-Global Arguments least_fixpoint : simpl never.
-Definition greatest_fixpoint {A : Type}
-    (F : (A → Prop) → (A → Prop)) (x : A) : Prop :=
-  tc_opaque (∃ Φ : A -> Prop, (∀ x, Φ x → F Φ x) ∧ Φ x).
-Global Arguments greatest_fixpoint : simpl never.
+Global Arguments prop_least_fixpoint : simpl never.
 
 Section least.
   Context {A : Type} (F : (A → Prop) → (A → Prop)) `{!MonoPred F}.
 
-  (* TODO: What are good names for these lemmas that don't conflict with the iris names? *)
-  Lemma pleast_fixpoint_unfold_2 x : F (least_fixpoint F) x → least_fixpoint F x.
+  Lemma prop_least_fixpoint_unfold_2 x : F (prop_least_fixpoint F) x → prop_least_fixpoint F x.
   Proof using Type*.
-    rewrite /least_fixpoint /=. move => HF Φ Hincl.
+    rewrite /prop_least_fixpoint /=. move => HF Φ Hincl.
     apply Hincl. apply: mono_pred; [|done].
     move => /= y Hy. apply Hy. done.
   Qed.
 
-  Lemma pleast_fixpoint_unfold_1 x : least_fixpoint F x → F (least_fixpoint F) x.
+  Lemma prop_least_fixpoint_unfold_1 x : prop_least_fixpoint F x → F (prop_least_fixpoint F) x.
   Proof using Type*.
     move => HF. apply HF. move => y Hy /=. apply: mono_pred; [|done].
-    move => z Hz. by apply: pleast_fixpoint_unfold_2.
+    move => z Hz. by apply: prop_least_fixpoint_unfold_2.
   Qed.
 
-  Lemma pleast_fixpoint_unfold x : least_fixpoint F x ↔ F (least_fixpoint F) x.
-  Proof using Type*. split; eauto using pleast_fixpoint_unfold_1, pleast_fixpoint_unfold_2. Qed.
+  Lemma prop_least_fixpoint_unfold x : prop_least_fixpoint F x ↔ F (prop_least_fixpoint F) x.
+  Proof using Type*. split; eauto using prop_least_fixpoint_unfold_1, prop_least_fixpoint_unfold_2. Qed.
 End least.
 
 Section least.
   Context {A : Type} (F : (A → Prop) → (A → Prop)) `{!MonoPred F}.
 
-  Lemma pleast_fixpoint_ind (Φ : A → Prop) :
-    (∀ y, F Φ y → Φ y) → ∀ x, least_fixpoint F x → Φ x.
+  Lemma prop_least_fixpoint_ind (Φ : A → Prop) :
+    (∀ y, F Φ y → Φ y) → ∀ x, prop_least_fixpoint F x → Φ x.
   Proof using Type*. move => HΦ x HF. by apply: HF. Qed.
 
   Definition wf_pred_mono Φ : MonoPred (λ (Ψ : A → Prop) (a : A), Φ a ∧ F Ψ a).
@@ -193,15 +188,34 @@ Section least.
   Qed.
   Local Existing Instance wf_pred_mono.
 
-  Lemma pleast_fixpoint_ind_wf (Φ : A → Prop) :
-    (∀ y, F (least_fixpoint (λ Ψ a, Φ a ∧ F Ψ a)) y → Φ y) →
-    ∀ x, least_fixpoint F x → Φ x.
+  Lemma prop_least_fixpoint_ind_wf (Φ : A → Prop) :
+    (∀ y, F (prop_least_fixpoint (λ Ψ a, Φ a ∧ F Ψ a)) y → Φ y) →
+    ∀ x, prop_least_fixpoint F x → Φ x.
   Proof using Type*.
-    move => Hmon x. rewrite pleast_fixpoint_unfold => Hx.
+    move => Hmon x. rewrite prop_least_fixpoint_unfold => Hx.
     apply Hmon. apply: mono_pred; [|done].
-    apply pleast_fixpoint_ind => y Hy.
-    rewrite pleast_fixpoint_unfold. split; [|done].
+    apply prop_least_fixpoint_ind => y Hy.
+    rewrite prop_least_fixpoint_unfold. split; [|done].
     by apply: Hmon.
+  Qed.
+End least.
+
+Section least.
+  Context {A B : Type} (F : ((A * B) → Prop) → ((A * B) → Prop)) `{!MonoPred F}.
+
+  Lemma prop_least_fixpoint_pair_ind (Φ : A → B → Prop) :
+    (∀ y1 y2, F (uncurry Φ) (y1, y2) → Φ y1 y2) → ∀ x1 x2, prop_least_fixpoint F (x1, x2) → Φ x1 x2.
+  Proof using Type*.
+    move => ? x1 x2. change (Φ x1 x2) with ((uncurry Φ) (x1, x2)).
+    apply prop_least_fixpoint_ind; [done|]. move => [??] /=. naive_solver.
+  Qed.
+
+  Lemma prop_least_fixpoint_pair_ind_wf (Φ : A → B → Prop) :
+    (∀ y1 y2, F (prop_least_fixpoint (λ Ψ a, uncurry Φ a ∧ F Ψ a)) (y1, y2) → Φ y1 y2) →
+    ∀ x1 x2, prop_least_fixpoint F (x1, x2) → Φ x1 x2.
+  Proof using Type*.
+    move => ? x1 x2. change (Φ x1 x2) with ((uncurry Φ) (x1, x2)).
+    apply prop_least_fixpoint_ind_wf; [done|]. move => [??] /=. naive_solver.
   Qed.
 End least.
 
