theories/asm.v
@@ -59,7 +59,7 @@ Lemma asm_step_WriteReg_i r f es rs ins:
   TStepI asm_module (AsmState (Some (WriteReg r f::es)) rs ins)
             (λ G, G true None (λ G', is_Some (rs !! r) ∧ G' (AsmState (Some (es)) (<[r:=f rs]>rs) ins))).
 Proof.
-  constructor => ? ?. apply TDStep => ???. left.
+  constructor => ? ?. apply steps_impl_step_end => ???.
   invert_all @m_step. eexists _. split; [done|].
   move => ? /=. naive_solver.
 Qed.
@@ -84,7 +84,7 @@ Lemma asm_step_Jump_i rs ins:
             G true (Some (EAJump pc rs)) (λ G', G' (AsmState None (rs) ins))
    ).
 Proof.
-  constructor => ? HG. apply TDStep => ???. left.
+  constructor => ? HG. apply steps_impl_step_end => ???.
   invert_all @m_step; specialize (HG _ ltac:(done)); simplify_option_eq.
   all: eexists _; split; [done|]; naive_solver.
 Qed.
@@ -112,7 +112,7 @@ Lemma asm_step_None_i rs ins:
       G true (Some (EARecvJump pc rs')) (λ G', G' (AsmState (Some i) rs' ins))
    ).
 Proof.
-  constructor => ? HG. apply TDStep => ???. left.
+  constructor => ? HG. apply steps_impl_step_end => ???.
   invert_all @m_step. eexists _. split; [naive_solver|]. naive_solver.
 Qed.
 Global Hint Resolve asm_step_None_i : tstep.
