theories/seq_product.v
@@ -275,7 +275,7 @@ Qed.
 Lemma mod_seq_product_step_None_i {EV1 EV2} (m1 : module EV1) (m2 : module EV2) σ1 σ2:
   TStepI (mod_seq_product m1 m2) (SPNone, σ1, σ2) (λ G, ∀ s, G true (Some (SPENone s)) (λ G', G' (s, σ1, σ2))).
 Proof.
-  constructor => G HG. apply: TDStep => ???. invert_all @m_step. left.
+  constructor => G HG. apply: steps_impl_step_end => ???. invert_all @m_step.
   eexists _. split; [done|]. naive_solver.
 Qed.
 Global Hint Resolve mod_seq_product_step_None_i : tstep.
@@ -286,7 +286,7 @@ Lemma mod_seq_product_step_l_i {EV1 EV2} (m1 : module EV1) (m2 : module EV2) σ1
      G b ((λ e, SPELeft e s') <$> κ) (λ G', P' (λ x, G' (s', x, σ2))))).
 Proof.
   constructor => G /tstepi_proof HP.
-  apply: (thas_trace_dual_submodule _ (mod_seq_product _ _) (λ x, (SPLeft, x, σ2))); [done| |].
+  apply: (steps_impl_submodule _ (mod_seq_product _ _) (λ x, (SPLeft, x, σ2))); [done| |].
   - move => ?? /= [?[HG HG']]. eexists _. split; [by apply HG|] => ? /= /HG'[?[??]]. naive_solver.
   - move => ????. invert_all' @m_step; simplify_eq/=; eexists _, _.
     split_and!; [done| |naive_solver].
@@ -300,7 +300,7 @@ Lemma mod_seq_product_step_r_i {EV1 EV2} (m1 : module EV1) (m2 : module EV2) σ1
      G b ((λ e, SPERight e s') <$> κ) (λ G', P' (λ x, G' (s', σ1, x))))).
 Proof.
   constructor => G /tstepi_proof HP.
-  apply: (thas_trace_dual_submodule _ (mod_seq_product _ _) (λ x, (SPRight, σ1, x))); [done| |].
+  apply: (steps_impl_submodule _ (mod_seq_product _ _) (λ x, (SPRight, σ1, x))); [done| |].
   - move => ?? /= [?[HG HG']]. eexists _. split; [by apply HG|] => ? /= /HG'[?[??]]. naive_solver.
   - move => ????. invert_all' @m_step; simplify_eq/=; eexists _, _.
     split_and!; [done| |naive_solver].
